SmallModel.v
@@ -1,0 +1,620 @@
+Require Import Coq.Strings.String.
+Require Import Coq.Init.Datatypes.
+Require Import Coq.Lists.List.
+Require Import Coq.micromega.Lia.
+Require Import Coq.ZArith.ZArith.
+Require Import coqutil.Semantics.OmniSmallstepCombinators.
+Require Import coqutil.Map.Interface.
+Require Import coqutil.Tactics.Tactics.
+Require Import coqutil.Word.Interface.
+Require Coq.Strings.HexString.
+Import ListNotations.
+Local Open Scope Z_scope.
+
+(*** Simplistic machine. ***)
+(* This is intended for quick prototyping. The machine has just a few
+   registers and instructions; it has neither memory nor flags. *)
+
+Section Registers.
+  (* General data registers, 32 bits each. *)
+  (* x0 is always wired to 0, x1 is the call stack. *)
+  Inductive gpr : Type :=
+  | x0 | x1 | x2 | x3 | x4 | x5 | x6 | x7.
+
+  (* Control and status registers, 32-bits each. *)
+  Inductive csr : Type :=
+  | CSR_RND
+  .
+
+  (* Catchall type indicating any register. *)
+  Inductive reg :=
+  | gpreg : gpr -> reg
+  | csreg : csr -> reg
+  .
+End Registers.
+
+Section ISA.
+  (* Straightline instructions (no control flow) *)
+  Inductive sinsn : Type :=
+  | Addi : gpr -> gpr -> Z -> sinsn
+  | Add : gpr -> gpr -> gpr -> sinsn
+  | Csrrs : csr -> gpr -> sinsn
+  .
+
+  (* Control-flow instructions *)
+  Inductive cinsn {addr : Type} : Type :=
+  (* TODO: technically ret is a special case of JALR, but only RET is used in practice *)
+  | Ret : cinsn
+  | Ecall : cinsn
+  | Jal : gpr -> addr -> cinsn
+  | Bne : gpr -> gpr -> addr -> cinsn
+  | Beq : gpr -> gpr -> addr -> cinsn
+  | Loop : gpr -> nat -> cinsn
+  | Loopi : nat -> nat -> cinsn
+  .
+
+  Inductive insn {addr : Type} : Type :=
+  | Straightline : sinsn -> insn
+  | Control : cinsn (addr:=addr) -> insn
+  .
+
+End ISA.
+
+(* Boilerplate definitions for comparing registers. *)
+Section RegisterEquality.
+  Local Ltac derive_eqb r1 r2 :=
+    pose r1 as x1;
+    pose r2 as x2;
+    destruct r1, r2;
+    lazymatch goal with
+    | x1 := ?x, x2 := ?x |- _ => clear; exact true
+    | _ => clear; exact false
+    end.
+  
+  Definition gpr_eqb (r1 r2 : gpr) : bool.
+  Proof. derive_eqb r1 r2. Defined.
+  Definition csr_eqb (r1 r2 : csr) : bool.
+  Proof. derive_eqb r1 r2. Defined.
+
+  Local Ltac prove_eqb_spec r1 r2 :=
+    destruct r1, r2; cbv [gpr_eqb]; constructor; congruence.
+  Lemma gpr_eqb_spec : forall r1 r2, BoolSpec (r1 = r2) (r1 <> r2) (gpr_eqb r1 r2).
+  Proof. prove_eqb_spec r1 r2. Qed.
+  Lemma csr_eqb_spec : forall r1 r2, BoolSpec (r1 = r2) (r1 <> r2) (csr_eqb r1 r2).
+  Proof. prove_eqb_spec r1 r2. Qed.
+End RegisterEquality.
+
+(* bitwise operation shorthand *)
+Local Infix "|'" := Z.lor (at level 40, only parsing) : Z_scope.
+Local Infix "&'" := Z.land (at level 40, only parsing) : Z_scope.
+Local Infix "<<" := Z.shiftl (at level 40, only parsing) : Z_scope.
+Local Infix ">>" := Z.shiftr (at level 40, only parsing) : Z_scope.
+Local Coercion Z.b2z : bool >-> Z.
+
+(* Executable model of OTBN. *)
+Section Exec.
+  (* Parameterize over the representation of code locations. *)
+  Context {addr : Type}
+    {advance_pc : addr -> addr}
+    {addr_eqb : addr -> addr -> bool}
+    {addr_eqb_spec : forall a1 a2, BoolSpec (a1 = a2) (a1 <> a2) (addr_eqb a1 a2)}.
+  Definition block (addr : Type) : Type := (list sinsn * option (cinsn (addr:=addr))).
+
+  (* error values for cases that should be unreachable (these can be
+     any value and exist mostly to help debugging -- it's easier to
+     understand that something went wrong when you see "error_Z" than
+     an unexpected 0). *)
+  Context {error_Z : Z}.
+
+  (* Parameterize over the map implementation. *)
+  Context {regfile : map.map reg Z} {blockmap : map.map addr (block addr)}.
+
+  (* Really, I want to talk about terminal states -- either a return
+     from the subroutine, the end of the program, or an error.
+
+     straightline needs/edits only regs, flags, dmem --> but can error
+     control needs/edits callstack, loopstack, pc, needs regs --> can also error 
+
+     need to process through, come out with a Prop in the end via cps style passing
+     the prop gives you rnd reasoning much easier
+   *)
+  Definition is_valid_addi_imm (imm : Z) : Prop :=
+    -2048 <= imm <= 2047.
+
+  Definition read_gpr (regs : regfile) (r : gpr) (P : Z -> Prop) : Prop :=
+    match r with
+    | x0 => P 0 (* x0 always reads as 0 *)
+    | x1 =>
+        (* TODO: call stack reads are rare in practice; for now, don't model *)
+        False
+    | _ => exists v, map.get regs (gpreg r) = Some v /\ P v
+    end.
+
+  Definition read_csr (regs : regfile) (r : csr) (P : Z -> Prop) : Prop :=
+    match r with
+    | CSR_RND => forall v, P v
+    end.
+
+  Definition cast32 (v : Z) : Z := v &' Z.ones 32.
+
+  Definition write_gpr (regs : regfile) (r : gpr) (v : Z) (P : regfile -> Prop) : Prop :=
+    match r with
+    | x0 => P regs
+    | x1 =>
+        (* TODO: this should push to the call stack, but is
+           practically never used. For now, don't model this behavior
+           and treat it as an error. *)
+        False
+    | _ => P (map.put regs (gpreg r) (cast32 v))
+    end.
+
+  Definition write_csr (regs : regfile) (r : csr) (v : Z) (P : regfile -> Prop) : Prop :=
+    match r with
+    | CSR_RND => P regs (* writes ignored *)
+    end.
+
+  Definition run1
+    (regs : regfile) (i : sinsn) (post : regfile -> Prop) : Prop :=
+    match i with
+    | Addi d x imm =>
+        is_valid_addi_imm imm /\
+          read_gpr regs x
+            (fun vx =>
+               write_gpr regs d (vx + imm) post)
+    | Add d x y =>
+        read_gpr regs x
+          (fun vx =>
+             read_gpr regs y
+               (fun vy =>
+                  write_gpr regs d (vx + vy) post))
+    | Csrrs d x =>
+        read_gpr regs x
+          (fun vx =>
+             read_csr regs d
+               (fun vd =>
+                  write_csr regs d (Z.lxor vd vx) post))
+    end.
+
+  Fixpoint run (regs : regfile) (sinsns : list sinsn) (post : regfile -> Prop) : Prop :=
+    match sinsns with
+    | [] => post regs
+    | i :: sinsns => run1 regs i (fun regs => run regs sinsns post)
+    end.
+
+  Fixpoint repeat_advance_pc (pc : addr) (n : nat) : addr :=
+    match n with
+    | O => pc
+    | S n => advance_pc (repeat_advance_pc pc n)
+    end.
+
+  Local Notation call_stack := (list addr) (only parsing).
+  Local Notation loop_stack := (list (addr * addr * nat)) (only parsing).
+  Inductive otbn_state : Type :=
+  | otbn_busy (pc : addr) (regs : regfile) (cstack : call_stack) (lstack : loop_stack)
+  | otbn_error (pc : addr) (errs : list string)
+  | otbn_done (pc : addr) (regs : regfile)
+  .  
+  Definition start_state (start_pc : addr) : otbn_state :=
+    otbn_busy start_pc map.empty [] [].
+  Definition get_pc (st : otbn_state) : addr :=
+    match st with
+    | otbn_busy pc _ _ _ => pc
+    | otbn_error pc _ => pc
+    | otbn_done pc _ => pc
+    end.
+  (* Pop an address off the call stack and jump to that location. *)
+  Definition call_stack_pop (st : otbn_state) (post : otbn_state -> Prop) : Prop :=
+    match st with
+    | otbn_busy pc regs cstack lstack =>
+        exists dst,
+        hd_error cstack = Some dst
+        /\ post (otbn_busy dst regs cstack lstack)
+    | _ => post st
+    end.
+  (* Push the next (one-advanced) PC onto the call stack. *)
+  Definition call_stack_push (st : otbn_state) (post : otbn_state -> Prop) : Prop :=
+    match st with
+    | otbn_busy pc regs cstack lstack =>
+        (length cstack < 8)%nat
+        /\ post (otbn_busy pc regs ((advance_pc pc) :: cstack) lstack)
+    | _ => post st
+    end.
+  Definition program_exit (st : otbn_state) (post : otbn_state -> Prop) : Prop :=
+    match st with
+    | otbn_busy pc regs cstack lstack => post (otbn_done pc regs)
+    | _ => post st
+    end.
+  Definition set_pc (st : otbn_state) (pc : addr) (post : otbn_state -> Prop) : Prop :=
+    match st with
+    | otbn_busy _ regs cstack lstack => post (otbn_busy pc regs cstack lstack)
+    | _ => post st
+    end.
+  Definition next_pc (st : otbn_state) (post : otbn_state -> Prop) : Prop :=
+    match st with
+    | otbn_busy pc regs cstack lstack => post (otbn_busy (advance_pc pc) regs cstack lstack)
+    | _ => post st
+    end.
+  Definition read_gpr_from_state (st : otbn_state) (r : gpr) (post : Z -> Prop) : Prop :=
+    match st with
+    | otbn_busy _ regs _ _ => read_gpr regs r post
+    | _ => False
+    end.
+
+  (* Begin a new loop. *)
+  Definition loop_start
+    (st : otbn_state) (iters : nat) (size : nat) (post : otbn_state -> Prop) : Prop :=
+    match st with
+    | otbn_busy pc regs cstack lstack =>
+        let start_pc := advance_pc pc in
+        let end_pc := repeat_advance_pc pc size in
+        (length lstack < 8)%nat
+        /\ post (otbn_busy start_pc regs cstack ((start_pc, end_pc, iters) :: lstack))
+    | _ => False
+    end.
+
+  (* Finish a loop iteration (and potentially the entire loop).
+    Expects that the current PC matches the loop-body end PC of the
+    first loop stack entry. *)
+  Definition loop_end (st : otbn_state) (post : otbn_state -> Prop) : Prop :=
+    match st with
+    | otbn_busy pc regs cstack lstack =>
+        exists start_addr end_addr iters,
+        hd_error lstack = Some (start_addr, end_addr, iters)
+        /\ end_addr = pc
+        /\ match iters with
+           | O => post (otbn_busy (advance_pc pc) regs cstack (tl lstack))
+           | S iters =>
+               post (otbn_busy start_addr regs cstack
+                       ((start_addr, end_addr, iters) :: tl lstack))
+           end
+    | _ => False
+    end.
+
+  (* TODO: is it possible to simplify the address logic here so we can
+    directly link "dst" as a block, even if it means repeated terms? *)
+  (* TODO: is it necessary to simulate some error conditions? There
+     should be a difference between "OTBN had an error", which
+     sometimes should in fact happen on some inputs, and "this program
+     is not valid" (e.g. out-of-bounds immediate value that cannot be
+     encoded). *)
+  Definition ctrl1 (st : otbn_state) (i : cinsn) (post : otbn_state -> Prop) : Prop :=
+    match i with
+    | Ret =>  call_stack_pop st post
+    | Ecall => program_exit st post
+    | Jal r dst =>
+        match r with
+        | x0 => set_pc st dst post
+        | x1 => call_stack_push st (fun st => set_pc st dst post)
+        | _ =>
+            (* technically it is possible to write the PC to other
+               registers but practically this is almost never done, so
+               for now we don't model it *)
+            False
+        end
+    | Bne r1 r2 dst =>
+        read_gpr_from_state st r1
+          (fun v1 =>
+             read_gpr_from_state st r2
+               (fun v2 =>
+                  (v1 = v2 /\ next_pc st post)
+                  \/ (v1 <> v2 /\ set_pc st dst post)))
+    | Beq r1 r2 dst =>
+        read_gpr_from_state st r1
+          (fun v1 =>
+             read_gpr_from_state st r2
+               (fun v2 =>
+                  (v1 <> v2 /\ next_pc st post)
+                  \/ (v1 = v2 /\ set_pc st dst post)))
+    | Loopi v n => loop_start st v n post
+    | Loop r n => read_gpr_from_state st r
+                    (fun v => 0 < v /\ loop_start st (Z.to_nat v) n post)
+    end.
+
+  Definition run_block (blocks : blockmap) (st : otbn_state)
+    (post : otbn_state -> Prop) : Prop :=
+    match st with
+    | otbn_busy pc regs cstack lstack =>
+        exists sinsns final,
+        map.get blocks pc = Some (sinsns, final)
+        /\ run regs sinsns
+             (fun regs =>
+                let pc := repeat_advance_pc pc (length sinsns) in
+                match final with
+                | Some i => ctrl1 st i post
+                | None => loop_end st post
+                end)
+    | _ => post st
+    end.
+End Exec.
+
+Section ErrorMonad.
+  (* returns either a value or an error message, helpful for debugging *)
+  Definition maybe (A : Type) : Type := A + string.
+  Definition bind {A B} (x : maybe A) (f : A -> maybe B) : maybe B :=
+    match x with
+    | inl a => f a
+    | inr err => inr err
+    end.
+  Definition map_err {A} (x : option A) (err : string) : maybe A :=
+    match x with
+    | Some v => inl v
+    | None => inr err
+    end.
+  Definition prefix_err {A} (x : maybe A) (prefix : string) : maybe A :=
+    match x with
+    | inl v => inl v
+    | inr err => inr (prefix ++ err)%string
+    end.
+  Definition maybe_map {A B} (f : A -> B) (x : maybe A) : maybe B :=
+    match x with
+    | inl v => inl (f v)
+    | inr err => inr err
+    end.
+  Fixpoint maybe_fold_left {A B} (f : A -> B -> maybe A) (l : list B) (x : A) : maybe A :=
+    match l with
+    | [] => inl x
+    | b :: l =>
+        bind (f x b) (maybe_fold_left f l)
+    end.
+  Definition assertion (cond : bool) (msg : string) : maybe unit :=
+    if cond then inl tt else inr msg.
+End ErrorMonad.
+Module ErrorMonadNotations.
+  Notation "a <- b ; c" := (bind b (fun a => c)) (at level 100, right associativity).
+  Notation Ok := inl (only parsing).
+  Notation "'Err' x" := (inr x%string) (at level 20, only parsing).
+End ErrorMonadNotations.
+
+Require Import coqutil.Map.SortedListZ.
+Require Import coqutil.Map.SortedListString.
+Local Coercion Straightline : sinsn >-> insn.
+Local Coercion Control : cinsn >-> insn.
+ 
+
+(* Contains a way to link programs into block maps. *)
+Section Build.
+  Definition advance_pc (pc : Z) := pc + 4.
+  Definition blockmap : map.map Z (block Z) := SortedListZ.map _.
+  Definition objects : map.map string (list (block string)) := SortedListString.map _.
+  Definition symbols : map.map string Z := SortedListString.map _.
+  Import ErrorMonadNotations.
+
+  (* Split a program at a given index in the instruction list and add
+     the label. Does nothing if the program is already split at this
+     index or the index is past the end of the program. *)
+  Fixpoint insert_label
+    (program : list (string * list (insn (addr:=string))))
+    (idx : nat) (label : string) : list (string * list (insn (addr:=string))) :=
+    match program with
+    | [] => program
+    | fn :: program =>
+        let name := fst fn in
+        let insns := snd fn in
+        if Nat.ltb idx (length insns)
+        then if Nat.eqb idx 0
+             then program
+             else
+               let fn1 := (name, firstn idx insns) in
+               let fn2 := (label, skipn idx insns) in
+               fn1 :: fn2 :: program
+        else fn :: insert_label program (idx - length insns) label
+    end.
+
+  Definition flatten_program (program : list (string * list (insn (addr:=string))))
+    : list (insn (addr:=string)) :=
+    fold_left (fun insns fn => insns ++ snd fn) program [].
+
+  (* Go through the program and add labels to the loop ends. *)
+  Definition label_loop_ends (program : list (string * list (insn (addr:=string))))
+    : list (string * list (insn (addr:=string))) :=
+    let insns := flatten_program program in
+    snd (fold_left
+           (fun lidx_program iidx =>
+              let lidx := fst lidx_program in
+              let program := snd lidx_program in
+              let i := nth_default (Ecall : insn) insns iidx in
+              let label := ("loop" ++ String.of_nat lidx ++ "_end")%string in
+              match i with
+              | Loop _ n =>
+                  let program := insert_label program (iidx + 1 + n) label in
+                  (S lidx, program)
+              | Loopi _ n =>
+                  let program := insert_label program (iidx + 1 + n) label in
+                  (S lidx, program)
+              | _ => (lidx, program)
+              end
+           )
+           (seq 0 (length insns)) (0%nat, program)).
+
+  Fixpoint get_blocks'
+    (insns : list (insn (addr:=string)))
+    (blocks : list (block string)) (curr : list sinsn)
+    : list (block string) :=
+    match insns with
+    | [] => match curr with
+            | [] => blocks
+            | _ => blocks ++ [(curr, None)]
+            end
+    | i :: insns =>
+        match i with
+        | Straightline i => get_blocks' insns blocks (curr ++ [i])
+        | Control i => get_blocks' insns (blocks ++ [(curr, Some i)]) []
+        end
+    end.
+  Definition get_blocks (insns : list (insn (addr:=string))) : list (block string) :=
+    get_blocks' insns [] [].
+
+  Definition get_objects (program : list (string * list (insn (addr:=string))))
+    : map.rep (map:=objects) :=
+    fold_left
+      (fun objs fn =>
+         let name := fst fn in
+         let insns := snd fn in
+         map.put objs name (get_blocks insns))
+      program map.empty.
+
+  (* Returns the PC at the end of IMEM plus the symbol table. *)
+  Definition get_symbols (program : list (string * list (insn (addr:=string)))) 
+    : Z * map.rep (map:=symbols) :=
+    fold_left
+      (fun (pc_syms : Z * (map.rep (map:=symbols))) fn =>
+         let pc := fst pc_syms in
+         let syms := snd pc_syms in
+         let name := fst fn in
+         let insns := snd fn in
+         let syms := map.put syms name pc in
+         let pc := repeat_advance_pc (advance_pc:=advance_pc) pc (length insns) in
+         (pc, syms))
+      program (0, map.empty).
+
+  Definition link_cinsn
+    (syms : map.rep (map:=symbols)) (i : cinsn (addr:=string)) : maybe (cinsn (addr:=Z)) :=
+    match i with
+    | Ret => Ok Ret
+    | Ecall => Ok Ecall
+    | Jal r dst =>
+        (dst <- map_err (map.get syms dst) ("Destination " ++ dst ++ " not found (jal)");
+         Ok (Jal r dst))
+    | Bne r1 r2 dst =>
+        (dst <- map_err (map.get syms dst) ("Destination " ++ dst ++ " not found (bne)");
+         Ok (Bne r1 r2 dst))
+    | Beq r1 r2 dst =>
+        (dst <- map_err (map.get syms dst) ("Destination " ++ dst ++ " not found (beq)");
+         Ok (Beq r1 r2 dst))
+    | Loop r n => Ok (Loop r n)
+    | Loopi imm n => Ok (Loopi imm n)
+    end.
+
+  Definition link_block (syms : map.rep (map:=symbols)) (b : block string) : maybe (block Z) :=
+    match snd b with
+    | None => Ok (fst b, None)
+    | Some i =>
+        (i <- link_cinsn syms i;
+         Ok (fst b, Some i))
+    end.
+
+  Definition block_size {addr} (b : block addr) : nat :=
+    length (fst b) + (match snd b with
+                      | None => 0
+                      | Some _ => 1
+                      end).
+
+  Fixpoint link_blocks
+    (syms : map.rep (map:=symbols)) (curr_blocks : list (block string))
+    (all_blocks : blockmap) (pc : Z) : maybe blockmap :=
+    match curr_blocks with
+    | [] => Ok all_blocks
+    | b :: curr_blocks =>
+        (b <- link_block syms b;
+         link_blocks syms curr_blocks
+           (map.put all_blocks pc b)
+           (repeat_advance_pc (advance_pc:=advance_pc) pc (block_size b)))
+    end.
+
+  (* TODO: the intermediate symbols won't be found here... maybe symbol + offset? *)
+  (* why do we need objs, given the shape program has already? Can we just skip it? *)
+  Definition link (objs : map.rep (map:=objects))
+    (syms : map.rep (map:=symbols)) : maybe blockmap :=
+    map.fold
+      (fun all_blocks name curr_blocks =>
+         (all_blocks <- all_blocks;
+          pc <- map_err (map.get syms name) ("Symbol " ++ name ++ " not found");
+          link_blocks syms curr_blocks all_blocks pc))
+      (Ok map.empty)
+      objs.
+
+  Definition build (program : list (string * list (insn (addr:=string))))
+    : maybe blockmap :=
+    let program := label_loop_ends program in
+    let objs := get_objects program in
+    let syms := snd (get_symbols program) in
+    link objs syms.
+End Build.
+
+Module Test.
+  (* TODO: the current method can't reason about individual functions
+  at all -- we get a call stack error, no? Maybe we can make proofs
+  that include "there's a PC in the call stack"? *)
+  
+  (* Test program 0 : a function that adds two registers.
+
+     start:
+       addi x2, x0, 2
+       addi x3, x0, 3
+       jal  x1, add
+       ecall
+
+     add:
+       add  x5, x2, x3
+       ret
+   *)
+  Definition test_program0 : list (string * list (insn (addr:=string))) :=
+    [ ("start",
+        [ (Addi x2 x0 2 : insn);
+          (Addi x3 x0 3 : insn);
+          (Jal x1 "add" : insn);
+          (Ecall : insn)]);
+      ("add",
+        [(Add x5 x2 x3 : insn);
+         (Ret : insn)])]%string.
+
+  (* Test program 1 : build multiplication out of addition
+
+     mul:
+       addi   x4, x0, x0
+       loop   x2, 2
+         jal    x1, add
+         addi   x4, x5, 0
+       ret
+
+     add:
+       add  x5, x2, x3
+       ret
+  *)
+  Definition test_program1 : list (string * list (insn (addr:=string))) :=
+    [ ("mul",
+        [ (Addi x4 x0 0 : insn);
+          (Loop x2 2 : insn);
+          (Jal x1 "add" : insn);
+          (Addi x4 x5 0 : insn);
+          (Ret : insn)]);
+      ("add",
+        [(Add x5 x2 x3 : insn);
+         (Ret : insn)])]%string.
+
+  Compute (label_loop_ends test_program0).
+  Compute (get_objects test_program0).
+  Compute (get_symbols test_program0).
+  Compute (build test_program0).
+  
+  Compute (label_loop_ends test_program1).
+  Compute (get_objects test_program1).
+  Compute (get_symbols test_program1).
+  Compute (build test_program1).
+
+  Ltac derive_blockmap program :=
+    let val := eval vm_compute in (build program) in
+    lazymatch val with
+    | inl ?x => exact x
+    | inr ?e => fail e
+    end.
+
+  Definition blocks0 : blockmap := ltac:(derive_blockmap test_program0).
+  Definition blocks1 : blockmap := ltac:(derive_blockmap test_program1).
+
+  Check eventually (run_block blocks0).
+  Print otbn_state.
+  Lemma test_program0_correct regfile :
+    map.ok regfile ->
+    forall (regs : regfile) a b,
+      map.get regs (gpreg x2) = Some a ->
+      map.get regs (gpreg x3) = Some b ->
+      eventually (run_block blocks0) regs
+  Proof.
+    cbv [test_blk_add]; intros.
+    rewrite run_block_step. cbv [run1].
+    eexists; split; [ eassumption | ].
+    eexists; split; [ eassumption | ].
+    cbv [write_gpr].
+  Qed.
+End Test.
